src/program_logic/staged_invariant.v
@@ -5,3 +5,4 @@ From Perennial.program_logic Require Export staged_invariant_use_idle.
 From Perennial.program_logic Require Export staged_invariant_use_inuse.
 From Perennial.program_logic Require Export staged_invariant_use_inuse2.
 From Perennial.program_logic Require Export staged_invariant_wpc_nval.
+From Perennial.program_logic Require Export staged_invariant_wp_nval.
